\documentclass[12pt]{amsart}

\textwidth = 6.2 in
\textheight = 8.5 in
\oddsidemargin = 0.0 in
\evensidemargin = 0.0 in
\topmargin = 0.0 in
\headheight = 0.0 in
\headsep = 0.3 in
\parskip = 0.05 in
\parindent = 0.3 in

\usepackage{enumerate}
\usepackage{amsmath}
\usepackage{color}
\def\cc{\color{blue}}
\usepackage[normalem]{ulem}
\usepackage{amsfonts, amsmath, amssymb, amsthm}
\usepackage{systeme}
\usepackage[none]{hyphenat}
\usepackage{graphicx}
\graphicspath{{./images/}}
\usepackage{esint}
\usepackage{cancel}

\title{Homework 2}
\author{Sai Sivakumar}

\begin{document}
\maketitle

For $n\in \mathbb{N}$, let $a_n = \sum_{j = 1}^n j^{-3}$. Prove by induction that $a_n \leq 2-\frac{1}{n^2}$ for all $n\in\mathbb{N}$.

\begin{proof}
    We use mathematical induction. Let $a_n = \sum_{j = 1}^n j^{-3}$ for $n\in\mathbb{N}$ be as given. Observe for $n = 1$, \[1 = a_1 \leq 1 = 2-\frac{1}{1^2}.\] Then suppose $n\in \mathbb{N}$ and $a_n\leq 2-\frac{1}{n^2}$, that is, $2-a_n \geq \frac{1}{n^2}$. It follows that \begin{align*}
        2-\frac{1}{(n+1)^2}-a_{n+1} &= \left( 2-a_n\right) -\frac{1}{(n+1)^2} - \frac{1}{(n+1)^3} \\
        &\geq \frac{1}{n^2}-\frac{1}{(n+1)^2} - \frac{1}{(n+1)^3} \\
        &= \frac{1}{n^2} - \frac{n+2}{(n+1)^3} \\
        &= \frac{(n+1)^3 - n^2(n+2)}{n^2(n+1)^3} \\
        &= \frac{n^2 + 3n+1}{n^2(n+1)^3},
    \end{align*} where we used the inductive hypothesis in writing the inequality. Since $n\geq 1$ ($n\in\mathbb{N}$), \[\frac{n^2 + 3n+1}{n^2(n+1)^3}\geq 0,\] which implies that \[2-\frac{1}{(n+1)^2}-a_{n+1} \geq 0.\] This is equivalent to writing \[a_{n+1}\leq 2-\frac{1}{(n+1)^2},\] and so by induction we have that $a_n\leq 2-\frac{1}{n^2}$ for all $n\in\mathbb{N}$.
\end{proof}

\end{document}