\documentclass[12pt]{amsart}

\textwidth = 6.2 in
\textheight = 8.5 in
\oddsidemargin = 0.0 in
\evensidemargin = 0.0 in
\topmargin = 0.0 in
\headheight = 0.0 in
\headsep = 0.3 in
\parskip = 0.05 in
\parindent = 0.3 in

\usepackage{enumerate}
\usepackage{amsmath}
\usepackage{color}
\def\cc{\color{blue}}
\usepackage[normalem]{ulem}
\usepackage{amsfonts, amsmath, amssymb, amsthm}
\usepackage{systeme}
\usepackage[none]{hyphenat}
\usepackage{graphicx}
\graphicspath{{./images/}}
\usepackage{esint}
\usepackage{cancel}
\usepackage{physics}

\title{Homework 4}
\author{Sai Sivakumar}

\newtheorem{theorem}            {Theorem}[section]
\newtheorem{proposition}        [theorem]{Proposition}

\begin{document}
\maketitle

Let, for $n\in \mathbb{N},$
\[
b_n = \frac{2n^2+1}{n^2-n-3}.
\]
Show  $(b_n)$ converges arguing  directly from the definition of convergence.
%[Suggestion: show $n^2-n-3 \ge \frac{1}{3}n^2.$]

\begin{proof}
Let $(b_n)_{n=1}^{\infty}$ be a sequence given by $b_n = (2n^2+1)/(n^2-n-3)$, for $n\in\mathbb{N}$. Observe that \[n^2-n-3-\frac{1}{3}n^2  = \frac{2}{3}n^2-n-3 = \frac{1}{3}(n-3)(2n+3) \geq 0\] as long as $n\geq 3$. This implies that for $n\geq 3$, $n^2-n-3 \geq \frac{1}{3}n^2.$

Then for every $\varepsilon>0$, choose, from an Archimedean property and the previous observation, $N\in \mathbb{N}$ such that $N > \max\left\{3, \frac{27}{\varepsilon}\right\}$. Then for all $n>N$, \begin{align*}
    \abs{b_n-2} = \abs{\frac{2n^2+1}{n^2-n-3} -2} &= \frac{2n+7}{n^2-n-3}&\quad (\text{positive, since }n > 3)\\
    &< \frac{2n+7n}{n^2-n-3} &\quad (9n > 2n+7 \text{, since }n > 3) \\
    &< \frac{3\cdot 9n}{n^2} &\quad (n^2-n-3 > \frac{1}{3}n^2 \text{ for }n > 3) \\
    &= \frac{27}{n}\\
    &< \frac{27}{N}&\quad (n > N)\\
    &< \varepsilon
\end{align*}
Hence $(b_n)$ converges, and its limit is $2$.
\end{proof}
\end{document}